sort/valtyping.v
@@ -4,46 +4,69 @@ Import ListNotations.
 Require Import Coq.Bool.Bool Lia.
 From DTSMPST Require Import sort.term sort.subst sort.eval sort.closure sort.typecheck sort.soundness sort.monotonicity sort.completeness.
 
-(* Value typing and neutral typing (corrected) *)
+
+(* Corrected vty / nty: neutrals use type `neutral` where needed *)
+
 Inductive vty (Γ : list whnf) : whnf -> whnf -> Prop :=
 | VT_StarTy  : vty Γ VStar VStar
 | VT_NatTy   : vty Γ VNat  VStar
 
-(* Π-formation: codomain is checked by instantiating the closure at fresh *)
-| VT_PiTy : forall A B vB,
-    vty Γ A VStar ->
-    clos_eval' B fresh vB ->
-    vty (A :: Γ) vB VStar ->
-    vty Γ (VPi A B) VStar
+(* Pi formation *)
+| VT_Pi : forall (Aterm Bterm : term) (vA : whnf),
+    infer Γ Aterm VStar ->
+    eval' (sem_env_of_ctx Γ) Aterm vA ->
+    infer (vA :: Γ) Bterm VStar ->
+    vty Γ (VPi vA (Cl (sem_env_of_ctx Γ) Bterm)) VStar
 
-(* Σ-formation, same “fresh” trick; codomain lives under the extended context *)
-| VT_SigmaTy : forall A B vB,
-    vty Γ A VStar ->
-    clos_eval' B fresh vB ->
-    vty (A :: Γ) vB VStar ->
-    vty Γ (VSigma A B) VStar
+(* Sigma formation *)
+| VT_Sigma : forall (Aterm Bterm : term) (vA : whnf),
+    infer Γ Aterm VStar ->
+    eval' (sem_env_of_ctx Γ) Aterm vA ->
+    infer (vA :: Γ) Bterm VStar ->
+    vty Γ (VSigma vA (Cl (sem_env_of_ctx Γ) Bterm)) VStar
 
-(* λ : instantiate both the body-closure and codomain at fresh;
-   body must be typed under the extended context *)
-| VT_Lam : forall A B cl r vB,
-    vty Γ (VPi A B) VStar ->
+(* Lambda *)
+| VT_Lam : forall (Aterm Bterm : term) (cl : closure) (r vB vA : whnf),
+    vty Γ (VPi vA (Cl (sem_env_of_ctx Γ) Bterm)) VStar ->
     clos_eval' cl fresh r ->
-    clos_eval' B  fresh vB ->
-    vty (A :: Γ) r vB ->      (* <-- corrected: body types under A :: Γ *)
-    vty Γ (VLam cl) (VPi A B)
+    clos_eval' (Cl (sem_env_of_ctx Γ) Bterm) fresh vB ->
+    vty (vA :: Γ) r vB ->
+    vty Γ (VLam cl) (VPi vA (Cl (sem_env_of_ctx Γ) Bterm))
 
-(* Pair at a Σ-type: a : A and b : (B·a) *)
-| VT_Pair : forall (A : whnf) (Bcl : closure) (a b vB : whnf),
-    vty Γ A VStar ->
-    vty Γ a A ->
-    clos_eval' Bcl a vB ->
-    vty Γ b vB ->
-    vty Γ (VPair A vB a b) (VSigma A Bcl)
+(* Pair *)
+| VT_Pair : forall (Aterm Bterm : term) (a b vA vBsnd : whnf),
+    infer Γ Aterm VStar ->
+    eval' (sem_env_of_ctx Γ) Aterm vA ->
+    vty Γ a vA ->
+    clos_eval' (Cl (sem_env_of_ctx Γ) Bterm) a vBsnd ->
+    vty Γ b vBsnd ->
+    vty Γ (VPair vA vBsnd a b) (VSigma vA (Cl (sem_env_of_ctx Γ) Bterm))
 
 | VT_Zero  : vty Γ VZero VNat
 | VT_Succ  : forall n, vty Γ n VNat -> vty Γ (VSucc n) VNat
 
-(* Neutrals lift to values with the same type *)
+(* VEC: formation and constructors *)
+(* VVec n A is a type when A is a type and n is Nat *)
+| VT_Vec : forall (Aterm : term) (vA vn : whnf),
+    infer Γ Aterm VStar ->                       (* Aterm : ⋆ *)
+    eval' (sem_env_of_ctx Γ) Aterm vA ->        (* Aterm ⇓ vA *)
+    vty Γ vn VNat ->                             (* vn is a natural WHNF *)
+    vty Γ (VVec vn vA) VStar
+
+(* empty vector at A : Vec 0 A *)
+| VT_VNil : forall (Aterm : term) (vA : whnf),
+    infer Γ Aterm VStar ->
+    eval' (sem_env_of_ctx Γ) Aterm vA ->
+    vty Γ (VNilV vA) (VVec VZero vA)
+
+(* cons: A, n, x, xs are already semantic WHNFs *)
+| VT_VCons : forall (vA vn vx vxs : whnf),
+    vty Γ vA VStar ->                         (* A is a type *)
+    vty Γ vn VNat ->                          (* n : Nat (semantic) *)
+    vty Γ vx vA ->                            (* x : A *)
+    vty Γ vxs (VVec vn vA) ->                 (* xs : Vec n A *)
+    vty Γ (VConsV vA vn vx vxs) (VVec (VSucc vn) vA)
+
 | VT_Neutral : forall nx A, nty Γ nx A -> vty Γ (VNeutral nx) A
 
 with nty (Γ : list whnf) : neutral -> whnf -> Prop :=
@@ -51,45 +74,199 @@ with nty (Γ : list whnf) : neutral -> whnf -> Prop :=
     nth_error Γ i = Some A ->
     nty Γ (NVar i) A
 
-| NT_App  : forall n A B v vB,
-    nty Γ n (VPi A B) ->
-    vty Γ v A ->
-    clos_eval' B v vB ->
+| NT_App : forall (n : neutral) (vA : whnf) (Bcl : closure) (v vB : whnf),
+    nty Γ n (VPi vA Bcl) ->
+    vty Γ v vA ->
+    clos_eval' Bcl v vB ->
     nty Γ (NApp n v) vB
 
-| NT_Fst  : forall n A B,
-    nty Γ n (VSigma A B) ->
-    nty Γ (NFst n) A
+| NT_Fst  : forall (n : neutral) (vA : whnf) (Bcl : closure),
+    nty Γ n (VSigma vA Bcl) ->
+    nty Γ (NFst n) vA
 
-| NT_Snd  : forall n A B vB,
-    nty Γ n (VSigma A B) ->
-    clos_eval' B (VNeutral (NFst n)) vB ->
+| NT_Snd : forall (n : neutral) (vA : whnf) (Bcl : closure) (vB : whnf),
+    nty Γ n (VSigma vA Bcl) ->
+    clos_eval' Bcl (VNeutral (NFst n)) vB ->
     nty Γ (NSnd n) vB
 
-| NT_NatRec : forall P z s nx cP vTy,
-    vty Γ P (VPi VNat cP) ->
-    nty Γ nx VNat ->
+| NT_NatRec : forall (vP : whnf) z s (nx : neutral) (cP : closure) vTy,
+    vty Γ vP (VPi VNat cP) ->
+    nty Γ nx VNat ->                               (* nx is a neutral *)
     clos_eval' cP (VNeutral nx) vTy ->
-    nty Γ (NNatRec P z s nx) vTy
+    nty Γ (NNatRec vP z s nx) vTy
 
-| NT_VecRec : forall A P z s n nx cP c2 vTy,
-    vty Γ A VStar ->
-    vty Γ P (VPi VNat cP) ->
-    nty Γ nx (VVec n A) ->
-    clos_eval' cP n (VPi (VVec n A) c2) ->
+| NT_VecRec : forall (vA vP vz vs vn : whnf) (nx : neutral) (cP c2 : closure) vTy,
+    vty Γ vA VStar ->
+    vty Γ vP (VPi VNat cP) ->
+    nty Γ nx (VVec vn vA) ->
+    clos_eval' cP vn (VPi (VVec vn vA) c2) ->
     clos_eval' c2 (VNeutral nx) vTy ->
-    nty Γ (NVecRec A P z s n nx) vTy.
+    nty Γ (NVecRec vA vP vz vs vn nx) vTy.
 
-(* Theorem preservation_infer_bigstep :
+Lemma clos_evalk_sound :
+  forall k cl v, clos_evalk k cl = Some v -> clos_eval' cl fresh v.
+Proof.
+  intros; simpl in *.
+  unfold clos_evalk in *.
+  destruct cl.
+  eapply evalk_sound in H. easy.
+Qed.
+
+(* Lemma evfp1: forall k Γ t1 t2 t3 t4,
+  evalk k Γ (Pair t1 t2 t3 t4) = Some VStar -> False.
+Proof. intro k.
+       induction k; intros.
+       - easy.
+       - simpl in H.
+         case_eq(evalk k Γ t1); intros.
+         rewrite H0 in H.
+         case_eq(evalk k Γ t2); intros.
+         rewrite H1 in H.
+         case_eq(evalk k Γ t3); intros.
+         rewrite H in H.
+         eapply IHk. 
+ *)
+Lemma peq1: forall k Γ t w0 w1 w2 w3 v,
+  evalk k Γ t = Some (VPair w1 w2 w3 v) ->
+  evalk k Γ (TFst t) = Some w0 ->
+  w0 = w3.
+Proof. intro k.
+       induction k; intros.
+       - easy.
+       - simpl in H, H0.
+         destruct t; try easy.
+         * case_eq(evalk k Γ t1); intros.
+           rewrite H1 in H.
+           easy.
+           rewrite H1 in H. easy.
+         * case_eq(evalk k Γ t1); intros.
+           rewrite H1 in H.
+           easy.
+           rewrite H1 in H. easy.
+         * case_eq(evalk k Γ t); intros.
+           rewrite H1 in H.
+           easy.
+           rewrite H1 in H. easy.
+         * case_eq(evalk k Γ t1); intros.
+           rewrite H1 in H.
+           case_eq(evalk k Γ t2); intros.
+           rewrite H2 in H.
+           case_eq(evalk k Γ t3); intros.
+           rewrite H3 in H.
+           case_eq(evalk k Γ t4); intros.
+           rewrite H4 in H.
+           inversion H. subst.
+           case_eq(evalk k Γ (Pair t1 t2 t3 t4) ); intros.
+           rewrite H5 in H0. 
+           destruct w; try easy.
+           apply evalk_sound in H5.
+          
+(*            inversion H5.
+           subst.
+           
+           apply evalk_sound in H5.
+           inversion H5.
+           apply evalk_sound in H5.
+           inversion H5.
+           apply evalk_sound in H5.
+           inversion H5.
+           apply evalk_sound in H5.
+           inversion H5.
+          
+           apply evalk_sound in H5. *)
+           inversion H5. subst.
+           apply evalk_sound in H3.
+           specialize (eval'_det _ _ _ _ H3 H17); intros. subst. inversion H0. easy.
+
+(*            apply evalk_sound in H5.
+           inversion H5. *)
+(*            apply evalk_sound in H5.
+           inversion H5.
+           apply evalk_sound in H5.
+           inversion H5.
+           apply evalk_sound in H5.
+           inversion H5.
+           apply evalk_sound in H5.
+           inversion H5.
+           apply evalk_sound in H5.
+           inversion H5. *)
+           
+           rewrite H5 in H0. easy.
+           rewrite H4 in H. easy.
+           rewrite H3 in H. easy.
+           rewrite H2 in H. easy.
+           rewrite H1 in H. easy.
+         * case_eq(evalk k Γ t); intros.
+           rewrite H1 in H.
+           destruct w; try easy.
+           case_eq(evalk k Γ (TFst t)); intros.
+           rewrite H2 in H0.
+           destruct w; try easy.
+           inversion H. subst. inversion H0. subst.
+           apply evalk_sound in H2.
+           inversion H2. subst.
+           apply evalk_sound in H1.
+           specialize (eval'_det _ _ _ _ H1 H5); intros.
+           inversion H3.
+           subst. easy.
+           rewrite H2 in H0. easy.
+           rewrite H1 in H. easy.
+         * case_eq(evalk k Γ t); intros.
+           rewrite H1 in H.
+           destruct w; try easy.
+           case_eq(evalk k Γ (TSnd t)); intros.
+           rewrite H2 in H0.
+           destruct w; try easy.
+           inversion H. subst. inversion H0. subst.
+           apply evalk_sound in H2.
+           inversion H2.
+           subst.
+           apply evalk_sound in H1.
+           specialize (eval'_det _ _ _ _ H1 H5); intros.
+           inversion H3.
+           subst. easy.
+           rewrite H2 in H0. easy.
+           rewrite H1 in H. easy.
+Admitted.
+
+Corollary conv_complete_clo :
+  forall B B',
+    conv_clo B B' ->
+    exists k v v',
+      clos_eval_fuel k B  fresh = Some v /\
+      clos_eval_fuel k B' fresh = Some v' /\
+      conv_fuel k v v' = true.
+Proof. destruct conv_complete as [_ H]. exact H. Qed.
+
+(* Lemma conv_clo_app :
+  forall c1 c2 x v1 v2,
+    conv_clo c1 c2 ->
+    clos_eval' c1 x v1 ->
+    clos_eval' c2 x v2 ->
+    conv v1 v2.
+Proof. intros.
+       apply conv_complete_clo in H.
+       destruct H as (k,(va,(vb,(Ha,(Hb,Hc))))).
+       apply clos_eval_fuel_sound in Ha.
+       apply clos_eval_fuel_sound in Hb.
+       unfold clos_eval' in *.
+       destruct c1, c2.
+       
+       induction c1; intros.
+       case_eq c2; intros.
+       subst.
+       inversion H. subst. *)
+
+Theorem preservation_infer_bigstep :
   forall k Γ t A v,
      infer_fuel k Γ t = Some A ->
      evalk k (sem_env_of_ctx Γ) t = Some v ->
-     exists B, vty Γ v B /\ conv A B
+     exists B, vty Γ v B /\ exists k', conv_fuel k' A B = true
 with preservation_check_bigstep:
   forall k Γ t A v,
      check_fuel k Γ t A = true ->
      evalk k (sem_env_of_ctx Γ) t = Some v ->
-     exists B, vty Γ v B /\ conv A B.
+     exists B, vty Γ v B /\ exists k', conv_fuel k' A B = true.
 Proof. intro k.
        induction k; intros.
        - easy.
@@ -97,10 +274,10 @@ Proof. intro k.
          case_eq t; intros.
          * subst. inversion H. subst. inversion H0. subst.
            exists VStar. split. constructor.
-           constructor.
+           exists 1. easy.
          * subst. inversion H. subst. inversion H0. subst.
            exists VStar. split. constructor.
-           constructor.
+           exists 1. easy.
          * subst.
            case_eq(evalk k (sem_env_of_ctx Γ) t0); intros.
            rewrite H1 in H0.
@@ -114,18 +291,263 @@ Proof. intro k.
            case_eq w1; intros; subst; try easy.
            inversion H0. subst. inversion H. subst.
            rewrite H1 in H3. inversion H3. subst.
-           specialize(IHk _ _ _ _ H2 H1).
-           destruct IHk as (B, (HB1, HB2)).
-           inversion HB2. subst.
            exists VStar. split.
-           apply VT_PiTy with (vB := VStar).
-           easy. simpl.
-           apply infer_fuel_sound in H4.
-           inversion H4. subst.
-           constructor. unfold env_cons. unfold sem_env_of_ctx. simpl.
-           simpl. exists VStar. intros.
-           constructor. constructor.
+           apply VT_Pi with (Aterm := t0) (Bterm := t1).
+           apply infer_fuel_sound with (k:=k). easy.
+           apply evalk_sound with (k:=k). easy.
+           apply infer_fuel_sound with (k:=k). easy.
+           exists 1. easy.
            rewrite H4 in H. easy.
            rewrite H3 in H. easy.
            rewrite H2 in H. easy.
-           rewrite H1 in H0. easy. *)
+           rewrite H1 in H0. easy.
+         * subst.
+           case_eq(evalk k (sem_env_of_ctx Γ) t0); intros.
+           rewrite H1 in H0.
+           case_eq(infer_fuel k Γ t0); intros.
+           rewrite H2 in H.
+           case_eq w0; intros; subst; try easy.
+           case_eq(evalk k (sem_env_of_ctx Γ) t0); intros.
+           rewrite H3 in H.
+           case_eq(infer_fuel k (w0 :: Γ) t1); intros.
+           rewrite H4 in H.
+           case_eq w1; intros; subst; try easy.
+           inversion H0. subst. inversion H. subst.
+           rewrite H1 in H3. inversion H3. subst.
+           exists VStar. split.
+           apply VT_Sigma with (Aterm := t0) (Bterm := t1).
+           apply infer_fuel_sound with (k:=k). easy.
+           apply evalk_sound with (k:=k). easy.
+           apply infer_fuel_sound with (k:=k). easy.
+           exists 1. easy.
+           rewrite H4 in H. easy.
+           rewrite H3 in H. easy.
+           rewrite H2 in H. easy.
+           rewrite H1 in H0. easy.
+         * subst. inversion H. subst. inversion H0. subst.
+           exists VNat. split. constructor. exists 1. easy.
+         * subst.
+           case_eq( evalk k (sem_env_of_ctx Γ) t0); intros.
+           rewrite H1 in H0.
+           case_eq(check_fuel k Γ t0 VNat); intros.
+           rewrite H2 in H. inversion H. subst. inversion H0. subst.
+           specialize(preservation_check_bigstep _ _ _ _ _ H2 H1).
+           destruct preservation_check_bigstep as (B, (HB1,HB2)).
+           destruct HB2 as (k2, HB2).
+           apply conv_fuel_sound in HB2.
+           inversion HB2. subst.
+           exists VNat. split. constructor. easy.
+           exists 1. easy.
+           rewrite H2 in H. easy.
+           rewrite H1 in H0. easy.
+         * subst. easy.
+         * subst.
+           case_eq(evalk k (sem_env_of_ctx Γ) t0); intros.
+           rewrite H1 in H0.
+           destruct w; try easy.
+           case_eq(infer_fuel k Γ t0); intros.
+           rewrite H2 in H.
+           destruct w; try easy.
+           inversion H. subst. inversion H0. subst.
+
+           specialize(IHk _ _ _ _ H2 H1).
+           destruct IHk as (B, (HB1,HB2)).
+           inversion HB1. subst.
+           destruct HB2 as (k2, HB2).
+           apply conv_fuel_sound in HB2.
+           inversion HB2. subst.
+(*            
+           
+           rewrite H2 in H. easy.
+           case_eq(infer_fuel k Γ t0); intros.
+           rewrite H2 in H.
+           destruct w; try easy.
+           inversion H. subst. inversion H0. subst.
+           specialize(IHk _ _ _ _ H2 H1).
+           destruct IHk as (B, (HB1,HB2)).
+           inversion HB1. subst.
+           destruct HB2 as (k2, HB2).
+           apply conv_fuel_sound in HB2.
+           inversion HB2.
+           rewrite H2 in H. easy.
+
+           case_eq(infer_fuel k Γ t0); intros.
+           rewrite H2 in H.
+           destruct w0; try easy.
+           inversion H. subst. inversion H0. subst.
+           specialize(IHk _ _ _ _ H2 H1).
+           destruct IHk as (B, (HB1,HB2)).
+           inversion HB1. subst.
+           destruct HB2 as (k2, HB2).
+           apply conv_fuel_sound in HB2.
+           inversion HB2.
+           rewrite H2 in H. easy.
+
+           case_eq(infer_fuel k Γ t0); intros.
+           rewrite H2 in H.
+           destruct w0; try easy.
+           inversion H. subst. inversion H0. subst.
+           specialize(IHk _ _ _ _ H2 H1).
+           destruct IHk as (B, (HB1,HB2)).
+           inversion HB1. subst.
+           destruct HB2 as (k2, HB2).
+           apply conv_fuel_sound in HB2.
+           inversion HB2.
+           rewrite H2 in H. easy.
+
+           case_eq(infer_fuel k Γ t0); intros.
+           rewrite H2 in H.
+           destruct w; try easy.
+           inversion H. subst. inversion H0. subst.
+           specialize(IHk _ _ _ _ H2 H1).
+           destruct IHk as (B, (HB1,HB2)).
+           inversion HB1. subst.
+           destruct HB2 as (k2, HB2).
+           apply conv_fuel_sound in HB2.
+           inversion HB2.
+           rewrite H2 in H. easy.
+
+           case_eq(infer_fuel k Γ t0); intros.
+           rewrite H2 in H.
+           destruct w; try easy.
+           inversion H. subst. inversion H0. subst.
+           specialize(IHk _ _ _ _ H2 H1).
+           destruct IHk as (B, (HB1,HB2)).
+           inversion HB1. subst.
+           destruct HB2 as (k2, HB2).
+           apply conv_fuel_sound in HB2.
+           inversion HB2. subst. *)
+           exists w1. split. easy.
+           apply conv_complete_conv in H6.
+           easy.
+           rewrite H2 in H. easy.
+           rewrite H1 in H0. easy.
+         * subst.
+           case_eq(evalk k (sem_env_of_ctx Γ) t0); intros.
+           rewrite H1 in H0.
+           destruct w; try easy.
+           case_eq(infer_fuel k Γ t0); intros.
+           rewrite H2 in H.
+           destruct w; try easy.
+           case_eq(evalk k (sem_env_of_ctx Γ) (TFst t0)); intros.
+           rewrite H3 in H.
+           case_eq( clos_eval_fuel k c w0); intros.
+           rewrite H4 in H.
+           inversion H. subst. inversion H0. subst.
+           specialize(IHk _ _ _ _ H2 H1).
+           destruct IHk as (B, (HB1,HB2)).
+           inversion HB1. subst.
+           destruct HB2 as (k2, HB2).
+           apply conv_fuel_sound in HB2.
+           inversion HB2. subst.
+           exists w2. split. easy.
+           
+(*            rewrite H2 in H. easy.
+           case_eq(infer_fuel k Γ t0); intros.
+           rewrite H2 in H.
+           destruct w; try easy.
+           inversion H. subst. inversion H0. subst.
+           specialize(IHk _ _ _ _ H2 H1).
+           destruct IHk as (B, (HB1,HB2)).
+           inversion HB1. subst.
+           destruct HB2 as (k2, HB2).
+           apply conv_fuel_sound in HB2.
+           inversion HB2. subst. easy.
+           rewrite H2 in H. easy.
+           
+           case_eq(infer_fuel k Γ t0); intros.
+           rewrite H2 in H.
+           destruct w0; try easy.
+           inversion H. subst. inversion H0. subst.
+           specialize(IHk _ _ _ _ H2 H1).
+           destruct IHk as (B, (HB1,HB2)).
+           inversion HB1. subst.
+           destruct HB2 as (k2, HB2).
+           apply conv_fuel_sound in HB2.
+           inversion HB2. subst.
+           rewrite H2 in H. easy.
+
+           case_eq(infer_fuel k Γ t0); intros.
+           rewrite H2 in H.
+           destruct w0; try easy.
+           inversion H. subst. inversion H0. subst.
+           specialize(IHk _ _ _ _ H2 H1).
+           destruct IHk as (B, (HB1,HB2)).
+           inversion HB1. subst.
+           destruct HB2 as (k2, HB2).
+           apply conv_fuel_sound in HB2.
+           inversion HB2. subst.
+           rewrite H2 in H. easy.
+
+           case_eq(infer_fuel k Γ t0); intros.
+           rewrite H2 in H.
+           destruct w; try easy.
+           inversion H. subst. inversion H0. subst.
+           specialize(IHk _ _ _ _ H2 H1).
+           destruct IHk as (B, (HB1,HB2)).
+           inversion HB1. subst.
+           destruct HB2 as (k2, HB2).
+           apply conv_fuel_sound in HB2.
+           inversion HB2. subst. easy.
+           rewrite H2 in H. easy.
+
+           case_eq(infer_fuel k Γ t0); intros.
+           subst.
+           rewrite H2 in H.
+           destruct w0; try easy.
+           case_eq(evalk k (sem_env_of_ctx Γ) (TFst t0)); intros.
+           rewrite H3 in H.
+           case_eq(clos_eval_fuel k c w); intros.
+           rewrite H4 in H.
+           inversion H. subst. inversion H0. subst.
+           specialize(IHk _ _ _ _ H2 H1).
+           destruct IHk as (B, (HB1,HB2)).
+           inversion HB1. subst.
+           destruct HB2 as (k2, HB2).
+           apply conv_fuel_sound in HB2.
+           inversion HB2. subst.
+           exists w1. split. easy. *)
+           apply clos_eval_fuel_sound in H4.
+           specialize(peq1 _ _ _ _ _ _ _ _ H1 H3); intros.
+           subst.
+           
+           inversion H15. subst.
+           specialize(H5 _ _ _ H4 H13).
+           apply conv_complete in H5. easy.
+           
+           rewrite H4 in H. easy.
+           rewrite H3 in H. easy.
+           rewrite H2 in H. easy.
+           rewrite H1 in H0. easy.
+         * subst.
+           admit.
+         * subst.
+           easy.
+         * subst.
+           case_eq(evalk k (sem_env_of_ctx Γ) t0); intros.
+           rewrite H1 in H0.
+           case_eq( evalk k (sem_env_of_ctx Γ) t1); intros.
+           rewrite H2 in H0.
+           case_eq(infer_fuel k Γ t0); intros.
+           rewrite H3 in H.
+           destruct w1; try easy.
+           rewrite H2 in H.
+           case_eq(check_fuel k Γ t1 w1); intros.
+           rewrite H4 in H.
+           case_eq(clos_eval_fuel k c w0 ); intros.
+           rewrite H5 in H.
+           inversion H. subst.
+           apply vappk_sound in H0.
+           inversion H0. subst.
+           specialize(IHk _ _ _ _ H3 H1).
+           destruct IHk as (B, (HB1,HB2)).
+           inversion HB1. subst.
+           destruct HB2 as (k2, HB2).
+           apply conv_fuel_sound in HB2.
+           inversion HB2. subst.
+           inversion H16. subst.
+           unfold clos_eval' in H9.
+           admit.
+           
+Admitted.
+
